

Linear distinct fractions

$$\int \frac{x^2 + 1}{(x-1)(x-2)(x-3)}$$

$$x(x-1)^2 \rightarrow \text{reducible}$$

$$x(x^2+1) \rightarrow \text{irreducible}$$

$$\frac{A}{x-1} + \frac{B}{x-2} + \frac{C}{x-3} = \frac{x^2+1}{(x-1)(x-2)(x-3)}$$

$$A(x-2)(x-3) + B(x-1)(x-3) + C(x-1)(x-2) = x^2+1$$

$$\underline{Ax^2 - 5Ax + 6A} + \underline{Bx^2 - 4Bx + 3B} + \underline{Cx^2 - 3Cx + 2C} = x^2 + 1$$

$$x^2 \text{ ppl: } A + B + C = 1$$

$$x \text{ ppl: } -5A - 4B - 3C = 0$$

$$\text{const: } 6A + 3B + 2C = 1$$

$$\text{REF: } A = 1 \quad B = -5 \quad C = 5$$

$$\int \frac{1}{x-1} - \frac{5}{x-2} + \frac{5}{x-3} dx = \ln|x-1| - 5\ln|x-2| + 5\ln|x-3| + C$$

$$\int \frac{1}{x-1} + \frac{1}{3x+1} dx = \ln|x-1| + \frac{1}{3}\ln|3x+1|$$

2X

$$\int \frac{2x^3 - 4x^2 - x - 3}{x^2 - 2x - 3} dx$$

$$\begin{array}{r} x^2 - 2x - 3 \overline{) 2x^3 - 4x^2 - x - 3} \\ \underline{- 2x^3 + 4x^2 - 6x} \phantom{- 3} \\ 5x - 3 \end{array}$$

$$\int 2x + \frac{5x - 3}{x^2 - 2x - 3} \rightarrow (x-3)(x+1)$$

$$\frac{A}{x-3} + \frac{B}{x+1}$$

$$A(x+1) + B(x-3) = 5x-3$$

$$Ax + A + Bx - 3B = 5x - 3$$

$$\text{coeff: } A + B = 5$$

$$\text{const: } A - 3B = -3$$

$$\begin{pmatrix} 1 & 1 & 5 \\ 1 & -3 & -3 \end{pmatrix} \rightarrow \begin{pmatrix} 1 & 0 & 3 \\ 0 & 1 & 2 \end{pmatrix}$$

$$A = 3, B = 2$$

$$\int 2x + \frac{3}{x-3} + \frac{2}{x+1} dx$$

$$x^2 + 3 \ln(x-3) + 2 \ln(x+1)$$

$$\frac{1}{2} + \frac{1}{3} + \frac{1}{9} = \frac{1}{18}$$

$$1 \cdot 9 + 1 \cdot (2 \cdot 3) + 1 \cdot 2$$

$$\int \frac{6x+7}{(x+2)^2} dx \quad \frac{6x+7}{(x+2)^2} = \frac{A}{x+2} + \frac{B}{(x+2)^2}$$

$$6x+7 = A(x+2) + B$$

$$Ax + 2A + B = 6x + 7$$

$$x \text{ coeff: } A = 6$$

$$\text{const: } 7 = 2A + B$$

$$B = -5$$

$$\int \frac{6}{x+2} - \frac{5}{(x+2)^2} dx$$

$$6 \ln |x+2|$$

$$u = x+2$$

$$du = dx$$

$$\begin{aligned} \rightarrow \int \frac{1}{(x+2)} dx &= -5 \int u^{-2} du \\ &= -5 \frac{u^{-1}}{-1} \\ &= \frac{5}{u} \end{aligned}$$